gen_global_rel -> globalbij

theories/simplang/globalbij.v
@@ -2,37 +2,39 @@ From simuliris.simulation Require Import slsls lifting.
 From simuliris.simplang Require Import proofmode tactics.
 From simuliris.simplang Require Import parallel_subst primitive_laws gen_log_rel gen_val_rel.
 
-(** * Generic relation for global variables
+(** * Bijection between global variables
 
-This file defines [gen_global_rel] that relates the global variables
-of source and target. It is used to prove the reflexivity of
-[GlobalVar x]. *)
+This file defines [globalbij] that asserts that all global variables
+are related via a [loc_rel] chosen by the user. It is used to prove
+the reflexivity of [GlobalVar x]. *)
 
-Section gen_global_rel.
+Section globalbij.
   Context `{!sheapGS Σ} `{!sheapInv Σ}.
-  Context (loc_rel : loc → loc → iProp Σ).
+  Context (loc_rel : loc → loc → iProp Σ) `{!∀ l_t l_s, Persistent (loc_rel l_t l_s)}.
   Context (thread_own : thread_id → iProp Σ).
   Let log_rel := (gen_log_rel loc_rel thread_own).
 
-  Definition gen_global_rel (g_t g_s : gset string) : iProp Σ :=
-    ⌜g_s ⊆ g_t⌝ ∗ target_globals g_t ∗ source_globals g_s ∗
+  Definition globalbij : iProp Σ :=
+     ∃ g_t g_s, ⌜g_s ⊆ g_t⌝ ∗ target_globals g_t ∗ source_globals g_s ∗
      [∗ set] g∈g_s, loc_rel (global_loc g) (global_loc g).
 
-  Global Instance gen_global_rel_persistent g_t g_s `{!∀ l_t l_s, Persistent (loc_rel l_t l_s)}:
-    Persistent (gen_global_rel g_t g_s).
+  Global Instance globalbij_persistent: Persistent globalbij.
   Proof. apply _. Qed.
 
-  Definition gen_global_rel_law : Prop :=
-    (∀ Φ, (∀ g_t g_s, gen_global_rel g_t g_s -∗ Φ) -∗ update_si Φ).
+  Definition sheap_inv_contains_globalbij : Prop :=
+    ∀ P_s σ_s T_s, sheap_inv P_s σ_s T_s -∗ globalbij.
 
   Lemma source_red_global' n Ψ π :
-    gen_global_rel_law →
+    sheap_inv_contains_globalbij →
     (target_global n -∗ source_global n -∗ loc_rel (global_loc n) (global_loc n) -∗
-                   source_red #(global_loc n) π Ψ) -∗
+       source_red #(global_loc n) π Ψ) -∗
     source_red (GlobalVar n) π Ψ.
   Proof.
     iIntros (Hrel) "Hred".
-    iApply source_red_update_si. iApply Hrel. iIntros (g_t g_s) "(%Hsub&Hgs_t&Hgs_s&Hrel)".
+    iApply source_red_update_si.
+    iIntros (?????) "($&$&$&$&Hinv)". iDestruct (Hrel with "Hinv") as "#Hbij".
+    iFrame. iModIntro.
+    iDestruct "Hbij" as (g_t g_s) "(%Hsub&Hgs_t&Hgs_s&Hrel)".
     iApply source_red_global. iIntros "#Hg_s".
     iDestruct (heap_global_in with "Hgs_s Hg_s") as %Hin. move: (Hin) => /Hsub?.
     iDestruct (heap_global_intro with "Hgs_t") as "#Hg_t"; [done|].
@@ -41,7 +43,7 @@ Section gen_global_rel.
   Qed.
 
   Lemma log_rel_global_var x :
-    gen_global_rel_law →
+    sheap_inv_contains_globalbij →
     ⊢ log_rel (GlobalVar x) (GlobalVar x).
   Proof.
     iIntros (Hrel ? xs) "!# Hs Ht"; simpl.
@@ -50,4 +52,4 @@ Section gen_global_rel.
     iApply target_red_sim_expr. iApply (target_red_global with "Hg_t"). iApply target_red_base. iModIntro.
     iApply sim_expr_base. iApply lift_post_val. iFrame.
   Qed.
-End gen_global_rel.
+End globalbij.
