theories/simplang/na_inv/inv.v
@@ -5,7 +5,7 @@ From simuliris.base_logic Require Export gen_sim_heap gen_sim_prog.
 From simuliris.simulation Require Import slsls lifting.
 From iris.algebra.lib Require Import gset_bij.
 From iris.base_logic.lib Require Import gset_bij.
-From simuliris.simplang Require Export class_instances primitive_laws heapbij gen_val_rel gen_log_rel gen_global_rel.
+From simuliris.simplang Require Export class_instances primitive_laws heapbij gen_val_rel gen_log_rel globalbij.
 From simuliris.simplang.na_inv Require Export na_locs.
 
 From iris.prelude Require Import options.
@@ -25,13 +25,13 @@ Section definitions.
     π ↪[ naGS_col_name ] col.
 
   Definition na_bij_interp (P_s : prog) (σ_s : state) (T_s : list expr) :=
-    (∃ L cols gs,
+    (∃ L cols,
         ⌜length cols = length T_s⌝ ∗
         ⌜na_locs_wf cols P_s σ_s T_s⌝ ∗
         ⌜na_locs_in_L cols L⌝ ∗
         ghost_map_auth naGS_col_name 1 (map_seq 0 cols) ∗
         heap_bij_interp L (λ _, alloc_rel_pred cols) ∗
-        gen_global_rel loc_rel gs gs)%I.
+        globalbij loc_rel)%I.
 End definitions.
 
 Section laws.
@@ -50,10 +50,10 @@ Section laws.
         ⌜∀ b' o' q, b' ≠ b_s → alloc_rel_pred cols (Loc b' o') q → alloc_rel_pred cols' (Loc b' o') q⌝ -∗
         ghost_map_auth naGS_col_name 1 (map_seq 0 cols') -∗ alloc_rel b_t b_s (λ _, alloc_rel_pred cols') -∗ na_bij_interp P_s σ_s' T_s').
   Proof.
-    iIntros "Hinv Hrel". iDestruct "Hinv" as (L cols ? ? ? HL) "(Hcols & Hbij & Hgs)".
+    iIntros "Hinv Hrel". iDestruct "Hinv" as (L cols ? ? HL) "(Hcols & Hbij & Hgs)".
     iExists _. do 2 (iSplit; [done|]). iFrame.
     iDestruct (heap_bij_access with "Hbij Hrel") as (?) "[$ Hclose]".
-    iIntros (cols' σ_s' T_s' ? ? Hdom HP) "Hcols He". iExists L, cols', _. iFrame. repeat (iSplit; [done|]).
+    iIntros (cols' σ_s' T_s' ? ? Hdom HP) "Hcols He". iExists L, cols'. iFrame. repeat (iSplit; [done|]).
     iSplit.
     { iPureIntro => ??????. efeed pose proof Hdom as Hd; [done.. | ].
       destruct Hd as [->|[?[??]]].
@@ -76,45 +76,41 @@ Section fix_heap.
     sheap_ext_rel π v_t v_s := na_locs π ∅ ∗ val_rel v_t v_s;
   |}%I.
   Next Obligation.
-    iIntros (????????) "(%L & %cols & %gs & % & % & ? &?)".
-    iExists _,_, _. iFrame. iPureIntro.
+    iIntros (????????) "(%L & %cols & % & % & ? &?)".
+    iExists _,_. iFrame. iPureIntro.
     rewrite insert_length. split; [done|].
     by apply: na_locs_wf_pure.
   Qed.
 
   Global Instance heap_bij_inv_supports_alloc : sheapInvSupportsAlloc.
   Proof.
-    constructor. iIntros (???????????) "(%L&%cols&%gs&%Hlen&%Hwf&?&?&?&?)".
-    iExists _,_, _. iFrame. iPureIntro. rewrite insert_length. split; [done|].
+    constructor. iIntros (???????????) "(%L&%cols&%Hlen&%Hwf&?&?&?&?)".
+    iExists _,_. iFrame. iPureIntro. rewrite insert_length. split; [done|].
     by apply: na_locs_wf_alloc.
   Qed.
   Global Instance heap_bij_inv_supports_free : sheapInvSupportsFree.
   Proof.
-    constructor. iIntros (???????????) "(%L&%cols&%gs&%Hlen&%Hwf&?&?&?&?)".
-    iExists _, _, _. iFrame. iPureIntro. rewrite insert_length. split; [done|].
+    constructor. iIntros (???????????) "(%L&%cols&%Hlen&%Hwf&?&?&?&?)".
+    iExists _, _. iFrame. iPureIntro. rewrite insert_length. split; [done|].
     by apply: na_locs_wf_free.
   Qed.
   Global Instance heap_bij_inv_supports_load o : sheapInvSupportsLoad o.
   Proof.
-    constructor. iIntros (?????????????) "(%L&%cols&%gs&%Hlen&%Hwf&?&?&?&?)".
-    iExists _, _, _. iFrame. iPureIntro. rewrite insert_length. split; [done|].
+    constructor. iIntros (?????????????) "(%L&%cols&%Hlen&%Hwf&?&?&?&?)".
+    iExists _, _. iFrame. iPureIntro. rewrite insert_length. split; [done|].
     by apply: na_locs_wf_load.
   Qed.
   Global Instance heap_bij_inv_supports_store : sheapInvSupportsStore Na1Ord.
   Proof.
-    constructor. iIntros (????????????) "(%L&%cols&%gs&%Hlen&%Hwf&?&?&?&?)".
-    iExists _, _, _. iFrame. iPureIntro. rewrite insert_length. split; [done|].
+    constructor. iIntros (????????????) "(%L&%cols&%Hlen&%Hwf&?&?&?&?)".
+    iExists _, _. iFrame. iPureIntro. rewrite insert_length. split; [done|].
     have [|??]:= lookup_lt_is_Some_2 cols π. { rewrite Hlen. by apply: lookup_lt_Some. }
     apply: na_locs_wf_store; [done | done | by left | done | done |done | done |done].
   Qed.
 
-  Lemma sim_bij_global_rel_law :
-    gen_global_rel_law loc_rel.
-  Proof.
-    iIntros (Φ) "HΦ".
-    iIntros (?????) "(HP_t & HP_s & Hσ_t & Hσ_s & (%L&%cols&%gs&?&?&?&?&?&#Hgs)) !>". iFrame.
-    iDestruct ("HΦ" with "Hgs") as "$". iExists _, _, _. by iFrame.
-  Qed.
+  Lemma sim_bij_contains_globalbij :
+    sheap_inv_contains_globalbij loc_rel.
+  Proof. by iIntros (???) "(%L&%cols&?&?&?&?&?&$)". Qed.
 
   Lemma sim_bij_exploit_store π l_t (l_s : loc) Φ e_s e_t col:
     (∀ P_s σ_s, reach_or_stuck P_s e_s σ_s (post_in_ectx (λ e' σ', ∃ v' : val, e' = Store Na1Ord #l_s v' ∧ σ' = σ_s))) →
@@ -311,10 +307,10 @@ Section fix_heap.
     iExists _, _. iSplit; [iPureIntro; by econstructor|].
     iMod (heap_write with "Hσ_s Hl") as "[$ ?]".
     iFrame. iModIntro.
-    iDestruct "Hinv" as "(%L&%cols&%gs&%Hlen&%Hwf&?&Hcols&?)".
+    iDestruct "Hinv" as "(%L&%cols&%Hlen&%Hwf&?&Hcols&?)".
     iDestruct (ghost_map_lookup with "Hcols Hc") as %Hcoll.
     rewrite lookup_map_seq_0 in Hcoll.
-    iDestruct ("Hsim" with "Hc [$]") as "$". iExists _, _, _. iFrame.
+    iDestruct ("Hsim" with "Hc [$]") as "$". iExists _, _. iFrame.
     iPureIntro. rewrite insert_length. split; [done|].
     apply: na_locs_wf_store; [done | done | by right | done | done | done | done |done].
   Qed.
@@ -434,7 +430,7 @@ Section fix_heap.
     iIntros (e_t' efs_t σ_t') "%"; inv_head_step.
     iExists _, _, _. iSplitR. { eauto with head_step. }
     simpl. iFrame.
-    iDestruct "Hinv" as (L cols gs Hlen Hwf ?) "(Hcols&[Hb HL]&Hgs)".
+    iDestruct "Hinv" as (L cols Hlen Hwf ?) "(Hcols&[Hb HL]&Hgs)".
     iMod (ghost_map_insert (length T_s) ∅ with "Hcols") as "[Hcols Hcol']".
     { apply lookup_map_seq_None. lia. }
     rewrite -Hlen -(map_seq_snoc 0).
@@ -444,7 +440,7 @@ Section fix_heap.
     iDestruct ("Hval" with "Hc") as "$".
     iSplitR "Hsim Hcol'"; last first.
     { iModIntro. iSplit; [|done]. iApply "Hsim". by rewrite Nat.add_0_r. }
-    iExists _, _, _. iFrame. iModIntro.
+    iExists _, _. iFrame. iModIntro.
     repeat iSplit; try iPureIntro.
     - rewrite !app_length insert_length /=. lia.
     - by apply na_locs_wf_fork.
@@ -469,14 +465,14 @@ Section fix_heap.
   Proof.
     iIntros (Hn Ht Hs) "[% Hs_t] [% Hs_s] Hl_t Hl_s Hval Hsim". iApply sim_update_si.
     iIntros (?????) "(HP_t & HP_s & Hσ_t & Hσ_s & Hinv)".
-    iDestruct "Hinv" as (L cols gs ? ? HL) "(Hcols & Hbij & Hgs)".
+    iDestruct "Hinv" as (L cols ? ? HL) "(Hcols & Hbij & Hgs)".
     iMod (heap_bij_insertN with "Hbij Hl_t Hl_s Hval Hs_t Hs_s") as "[Hbij #?]"; [done..| |].
     - move => o ? HLs. rewrite /alloc_rel_pred combine_na_locs_list_None //.
       move => π' cols' Hcols.
       destruct (cols' !! (l_s +ₗ o)) eqn: Hk => //.
       exfalso. have /=[??]:= HL _ _ _ _ Hcols Hk. by apply: HLs.
     - iModIntro. iDestruct ("Hsim" with "[//]") as "$". iFrame.
-      iExists _, _, _. iFrame. iPureIntro. split_and!; [done..|].
+      iExists _, _. iFrame. iPureIntro. split_and!; [done..|].
       by apply: na_locs_in_L_extend.
   Qed.
 
@@ -503,12 +499,12 @@ Section fix_heap.
     update_si Φ.
   Proof.
     iIntros "Hbij [% Hf] HΦ" (P_t σ_t P_s σ_s T_s) "($&$&$&$&Hinv)".
-    iDestruct "Hinv" as (L cols ????) "(?&Hb&?)".
+    iDestruct "Hinv" as (L cols ???) "(?&Hb&?)".
     case_match; [case_match|..].
     5: iDestruct (gen_val_rel_loc_source with "Hbij") as (? ->) "Hbij".
     5: iDestruct (heap_bij_block_size_ne with "Hbij Hf Hb") as %?.
     all: iModIntro; iDestruct ("HΦ" with "[//] [$Hf]") as "$"; [done|].
-    all: iExists _, _, _; by iFrame.
+    all: iExists _, _; by iFrame.
   Qed.
 
   Lemma sim_bij_freeable_ne l1 l_t2 l_s2 Φ n:
