theories/simplang/simple_inv/inv.v
@@ -4,7 +4,7 @@ From simuliris.base_logic Require Export gen_sim_heap gen_sim_prog.
 From simuliris.simulation Require Import slsls lifting.
 From iris.algebra.lib Require Import gset_bij.
 From iris.base_logic.lib Require Import gset_bij.
-From simuliris.simplang Require Export class_instances primitive_laws heapbij gen_val_rel gen_log_rel gen_global_rel.
+From simuliris.simplang Require Export class_instances primitive_laws heapbij gen_val_rel gen_log_rel globalbij.
 
 From iris.prelude Require Import options.
 
@@ -22,22 +22,18 @@ Section fix_heap.
 
   Global Program Instance simple_inv : sheapInv Σ := {|
     sheap_inv _ _ _:=
-      ∃ L gs,
+      ∃ L,
         heap_bij_interp L (λ _ _ q, q = Some 1%Qp) ∗
-        gen_global_rel loc_rel gs gs;
+        globalbij loc_rel;
     sheap_ext_rel _ := val_rel;
   |}%I.
   Next Obligation. done. Qed.
   Global Instance : sheapInvStateIndependent.
   Proof. done. Qed.
 
-  Lemma sim_bij_global_rel_law :
-    gen_global_rel_law loc_rel.
-  Proof.
-    iIntros (Φ) "HΦ".
-    iIntros (?????) "(HP_t & HP_s & Hσ_t & Hσ_s & (%L&%gs&Hinv&#Hgs)) !>". iFrame.
-    iDestruct ("HΦ" with "Hgs") as "$". iExists _, _. by iFrame.
-  Qed.
+  Lemma sim_bij_contains_globalbij :
+    sheap_inv_contains_globalbij loc_rel.
+  Proof. by iIntros (???) "(%L&?&$)". Qed.
 
   Lemma sim_bij_load_sc π l_t l_s Φ :
     l_t ↔h l_s -∗
@@ -46,7 +42,7 @@ Section fix_heap.
   Proof.
     iIntros "#[Hbij %Hidx] Hsim". destruct l_s as [b_s o], l_t as [b_t o']; simplify_eq/=.
     iApply sim_lift_head_step_both.
-    iIntros (??????) "[(HP_t & HP_s & Hσ_t & Hσ_s & (%L&%gs&Hinv&Hgs)) [% %Hsafe]]".
+    iIntros (??????) "[(HP_t & HP_s & Hσ_t & Hσ_s & (%L&Hinv&Hgs)) [% %Hsafe]]".
     have [l[v[m[[<-] Hsome]]]]:= pool_safe_irred _ _ _ _ _ _ _ Hsafe ltac:(done) ltac:(done).
     iPoseProof (heap_bij_access with "Hinv Hbij") as "(% & Halloc & Hclose)"; first last.
     iDestruct (alloc_rel_read true with "Halloc Hσ_s Hσ_t") as (????) "#?"; [done| naive_solver |]; simplify_eq.
@@ -56,7 +52,7 @@ Section fix_heap.
     iSplitR; first by eauto with head_step.
     iFrame => /=. rewrite right_id.
     iSplitR "Hsim".
-    - iExists L, gs. iFrame. by iApply "Hclose".
+    - iExists L. iFrame. by iApply "Hclose".
     - by iApply "Hsim".
   Qed.
 
@@ -67,7 +63,7 @@ Section fix_heap.
   Proof.
     iIntros "#[Hbij %Hidx] Hsim". destruct l_s as [b_s o], l_t as [b_t o']; simplify_eq/=.
     iApply sim_lift_head_step_both.
-    iIntros (??????) "[(HP_t & HP_s & Hσ_t & Hσ_s & (%L&%gs&Hinv&#Hgs)) [% %Hsafe]]".
+    iIntros (??????) "[(HP_t & HP_s & Hσ_t & Hσ_s & (%L&Hinv&#Hgs)) [% %Hsafe]]".
     have [l[v[m[[<-] Hsome]]]]:= pool_safe_irred _ _ _ _ _ _ _ Hsafe ltac:(done) ltac:(done).
     iPoseProof (heap_bij_access with "Hinv Hbij") as "(% & Halloc & Hclose)".
     iDestruct (alloc_rel_read true with "Halloc Hσ_s Hσ_t") as (????) "#Hv"; [done| naive_solver |]; simplify_eq.
@@ -78,7 +74,7 @@ Section fix_heap.
     iSplitR; first by eauto with head_step.
     iFrame => /=. rewrite right_id.
     iSplitR "Hsim".
-    - iExists L, gs. iFrame "Hgs". by iApply "Hclose".
+    - iExists L. iFrame "Hgs". by iApply "Hclose".
     - by iApply "Hsim".
   Qed.
 
@@ -89,7 +85,7 @@ Section fix_heap.
   Proof.
     iIntros "#[Hbij %Hidx] Hsim". destruct l_s as [b_s o], l_t as [b_t o']; simplify_eq/=.
     iApply sim_lift_head_step_both.
-    iIntros (??????) "[(HP_t & HP_s & Hσ_t & Hσ_s & (%L&%gs&Hinv&#Hgs)) [% %Hsafe]]".
+    iIntros (??????) "[(HP_t & HP_s & Hσ_t & Hσ_s & (%L&Hinv&#Hgs)) [% %Hsafe]]".
     have [l[v[m[[<-] Hsome]]]]:= pool_safe_irred _ _ _ _ _ _ _ Hsafe ltac:(done) ltac:(done).
     iPoseProof (heap_bij_access with "Hinv Hbij") as "(% & Halloc & Hclose)"; first last.
     iDestruct (alloc_rel_read true with "Halloc Hσ_s Hσ_t") as (????) "#Hv"; [done|naive_solver|]; simplify_eq.
@@ -100,7 +96,7 @@ Section fix_heap.
     iSplitR; first by eauto with head_step.
     iFrame => /=. rewrite right_id.
     iSplitR "Hsim".
-    - iExists _, gs. iFrame "Hgs". by iApply "Hclose".
+    - iExists _. iFrame "Hgs". by iApply "Hclose".
     - iApply sim_bij_load_na2; [|done]. by iSplit.
   Qed.
 
@@ -118,7 +114,7 @@ Section fix_heap.
   Proof.
     iIntros "#[Hbij %Hidx] Hval Hsim". destruct l_s as [b_s o], l_t as [b_t o']; simplify_eq/=.
     iApply sim_lift_head_step_both.
-    iIntros (??????) "[(HP_t & HP_s & Hσ_t & Hσ_s & (%L&%gs&Hinv&#Hgs)) [% %Hsafe]]".
+    iIntros (??????) "[(HP_t & HP_s & Hσ_t & Hσ_s & (%L&Hinv&#Hgs)) [% %Hsafe]]".
     have [l[v[[<-] Hsome]]]:= pool_safe_irred _ _ _ _ _ _ _ Hsafe ltac:(done) ltac:(done).
     iPoseProof (heap_bij_access with "Hinv Hbij") as "(% & Halloc & Hclose)".
     iDestruct (alloc_rel_read true with "Halloc Hσ_s Hσ_t") as (????) "#Hv"; [done|naive_solver|]; simplify_eq.
@@ -127,7 +123,7 @@ Section fix_heap.
     iMod (alloc_rel_write with "Halloc Hσ_s Hσ_t Hval") as "[Halloc [Hσ_s Hσ_t]]"; [done|naive_solver|].
     iModIntro. iExists _, _, _.
     iSplitR; first by eauto with head_step.
-    iFrame => /=. rewrite right_id. iExists _, gs. iFrame "Hgs". by iApply "Hclose".
+    iFrame => /=. rewrite right_id. iExists _. iFrame "Hgs". by iApply "Hclose".
   Qed.
 
   Lemma sim_bij_store_na2 π l_t l_s v_t v_s Φ :
@@ -138,7 +134,7 @@ Section fix_heap.
   Proof.
     iIntros "#[Hbij %Hidx] Hval Hsim". destruct l_s as [b_s o], l_t as [b_t o']; simplify_eq/=.
     iApply sim_lift_head_step_both.
-    iIntros (??????) "[(HP_t & HP_s & Hσ_t & Hσ_s & (%L&%gs&Hinv&#Hgs)) [% %Hsafe]]".
+    iIntros (??????) "[(HP_t & HP_s & Hσ_t & Hσ_s & (%L&Hinv&#Hgs)) [% %Hsafe]]".
     have [l[v[[<-] Hsome]]]:= pool_safe_irred _ _ _ _ _ _ _ Hsafe ltac:(done) ltac:(done).
     iPoseProof (heap_bij_access with "Hinv Hbij") as "(% & Halloc & Hclose)"; first last.
     iDestruct (alloc_rel_read true with "Halloc Hσ_s Hσ_t") as (????) "#Hv"; [done|naive_solver|]; simplify_eq.
@@ -147,7 +143,7 @@ Section fix_heap.
     iMod (alloc_rel_write with "Halloc Hσ_s Hσ_t Hval") as "[Halloc [Hσ_s Hσ_t]]"; [done|naive_solver|].
     iModIntro. iExists _, _, _.
     iSplitR; first by eauto with head_step.
-    iFrame => /=. rewrite right_id. iExists L, gs. iFrame "Hgs". by iApply "Hclose".
+    iFrame => /=. rewrite right_id. iExists L. iFrame "Hgs". by iApply "Hclose".
   Qed.
 
   Lemma sim_bij_store_na1 π l_t l_s v_t v_s Φ :
@@ -158,7 +154,7 @@ Section fix_heap.
   Proof.
     iIntros "#[Hbij %Hidx] Hval Hsim". destruct l_s as [b_s o], l_t as [b_t o']; simplify_eq/=.
     iApply sim_lift_head_step_both.
-    iIntros (??????) "[(HP_t & HP_s & Hσ_t & Hσ_s & (%L&%gs&Hinv&#Hgs)) [% %Hsafe]]".
+    iIntros (??????) "[(HP_t & HP_s & Hσ_t & Hσ_s & (%L&Hinv&#Hgs)) [% %Hsafe]]".
     have [l[v[[<-] Hsome]]]:= pool_safe_irred _ _ _ _ _ _ _ Hsafe ltac:(done) ltac:(done).
     iPoseProof (heap_bij_access with "Hinv Hbij") as "(% & Halloc & Hclose)"; first last.
     iDestruct (alloc_rel_read true with "Halloc Hσ_s Hσ_t") as (????) "#Hv"; [done|naive_solver|]; simplify_eq.
@@ -169,7 +165,7 @@ Section fix_heap.
     iSplitR; first by eauto with head_step.
     iFrame => /=. rewrite right_id.
     iSplitR "Hsim Hval".
-    - iExists _, gs. iFrame "Hgs". by iApply "Hclose".
+    - iExists _. iFrame "Hgs". by iApply "Hclose".
     - iApply (sim_bij_store_na2 with "[] Hval Hsim"). by iSplit.
   Qed.
 
@@ -187,7 +183,7 @@ Section fix_heap.
   Proof.
     iIntros "#[Hbij %Hidx] Hsim". destruct l_s as [b_s o], l_t as [b_t o']; simplify_eq/=.
     iApply sim_lift_head_step_both.
-    iIntros (??????) "[(HP_t & HP_s & Hσ_t & Hσ_s & (%L&%gs&Hinv&#Hgs)) [% %Hsafe]]".
+    iIntros (??????) "[(HP_t & HP_s & Hσ_t & Hσ_s & (%L&Hinv&#Hgs)) [% %Hsafe]]".
     have [m[?[[<-][[<-][?[??]]]]]]:= pool_safe_irred _ _ _ _ _ _ _ Hsafe ltac:(done) ltac:(done).
     iPoseProof (heap_bij_access with "Hinv Hbij") as "(% & Halloc & Hclose)"; first last.
     iMod (alloc_rel_free with "Halloc Hσ_s Hσ_t") as (??) "(Halloc & Hσ_s & Hσ_t)"; [done..|].
@@ -195,7 +191,7 @@ Section fix_heap.
     iIntros (e_t' efs σ_t') "%"; inv_head_step.
     iModIntro. iExists _, _, _.
     iSplitR; first by eauto with head_step.
-    iFrame. iSplit; [|done]. iExists L, gs. iFrame "Hgs". by iApply "Hclose".
+    iFrame. iSplit; [|done]. iExists L. iFrame "Hgs". by iApply "Hclose".
   Qed.
 
   Lemma sim_bij_insertN π l_t l_s vs_t vs_s e_t e_s n Φ :
@@ -211,9 +207,9 @@ Section fix_heap.
     e_t ⪯{π} e_s [{ Φ }].
   Proof.
     iIntros (Hn Ht Hs) "[% Hs_t] [% Hs_s] Hl_t Hl_s Hval Hsim". iApply sim_update_si.
-    iIntros (?????) "(HP_t & HP_s & Hσ_t & Hσ_s & (%L&%gs&Hinv&#Hgs))".
+    iIntros (?????) "(HP_t & HP_s & Hσ_t & Hσ_s & (%L&Hinv&#Hgs))".
     iMod (heap_bij_insertN with "Hinv Hl_t Hl_s Hval Hs_t Hs_s") as "[Hb #Ha]"; [done .. | ].
-    iModIntro. iFrame. iDestruct ("Hsim" with "[//]") as "$". iExists _, gs. by iFrame "Hgs".
+    iModIntro. iFrame. iDestruct ("Hsim" with "[//]") as "$". iExists _. by iFrame "Hgs".
   Qed.
 
   Lemma sim_bij_insert π l_t l_s v_t v_s e_t e_s Φ :
